@prefix rdf: <http://www.w3.org/1999/02/22-rdf-syntax-ns#> .
@prefix rdfs: <http://www.w3.org/2000/01/rdf-schema#> .
@prefix xsd: <http://www.w3.org/2001/XMLSchema#> .
@prefix owl: <http://www.w3.org/2002/07/owl#> .
@prefix geojson: <https://purl.org/geojson/vocab#> .
@prefix schema: <https://schema.org/> .
@prefix untp-core: <https://test.uncefact.org/vocabulary/untp/core/0/> .

#################### Classes

untp-core:Address a rdfs:Class ;
  rdfs:label "Address" ;
  rdfs:comment "A postal address." .

untp-core:Attestation a rdfs:Class ;
  rdfs:label "Attestation" ;
  rdfs:comment "A conformity attestation issued by a competent body that defines one or more assessments (eg carbon intensity) about a product (eg battery) against a specification (eg LCA method) defined in a standard or regulation." .

untp-core:BinaryFile a rdfs:Class ;
  rdfs:label "BinaryFile" ;
  rdfs:comment "A binary file reference including name and file type." .

untp-core:Characteristics a rdfs:Class ;
  rdfs:label "Characteristics" ;
  rdfs:comment "Extension point for commodity specific characteristics like battery capacity, clothing size, etc." .

untp-core:CircularityPerformance a rdfs:Class ;
  rdfs:label "CircularityPerformance" ;
  rdfs:comment "High level circularity information about this product.  Note that this does not substitute for detailed product circularity data sheet (PCDS) criteria which would be represented as a self-issued UNTP Digital Conformity Credential as a set of assessments against individual ISO PCDS criteria." .

untp-core:Claim a rdfs:Class ;
  rdfs:label "Claim" ;
  rdfs:comment "A declaration of conformance with one or more criteria from a specific standard or regulation.  " ;
  rdfs:subClassOf "untp-core:Declaration" .

untp-core:Classification a rdfs:Class ;
  rdfs:label "Classification" ;
  rdfs:comment "A classification scheme and code / name representing a category value for a product, entity, or facility." .

untp-core:ConformityScheme a rdfs:Class ;
  rdfs:label "ConformityScheme" ;
  rdfs:comment "A formal governance scheme under which this attestation is issued (eg ACRS structural steel certification)" .

untp-core:CredentialIssuer a rdfs:Class ;
  rdfs:label "CredentialIssuer" ;
  rdfs:comment "The issuer party (person or organisation) of a verifiable credential." .

untp-core:Criterion a rdfs:Class ;
  rdfs:label "Criterion" ;
  rdfs:comment "A specific rule or criterion within a standard or regulation. eg a carbon intensity calculation rule within an emissions standard." .

untp-core:Declaration a rdfs:Class ;
  rdfs:label "Declaration" ;
  rdfs:comment "A specific assessment about the product or facility against a specific specification.  Eg the carbon intensity of a given product or batch." .

untp-core:Dimension a rdfs:Class ;
  rdfs:label "Dimension" ;
  rdfs:comment "Overall (length, width, height) dimensions and weight/volume of an item." .

untp-core:EmissionsPerformance a rdfs:Class ;
  rdfs:label "EmissionsPerformance" ;
  rdfs:comment "Product specific characteristics.  This class is an extension point for industry specific product characteristics or performance information such as clothing size or battery capacity." .

untp-core:Endorsement a rdfs:Class ;
  rdfs:label "Endorsement" ;
  rdfs:comment "The authority under which a conformity claim is issued.  For example a national accreditation authority may authorise a test lab to issue test certificates about a product against a standard. " .

untp-core:Facility a rdfs:Class ;
  rdfs:label "Facility" ;
  rdfs:comment "The physical site (eg farm or factory) where the product or materials was produced." .

untp-core:IdentifierScheme a rdfs:Class ;
  rdfs:label "IdentifierScheme" ;
  rdfs:comment "An identifier registration scheme for products, facilities, or organisations. Typically operated by a state, national or global authority." .

untp-core:Link a rdfs:Class ;
  rdfs:label "Link" ;
  rdfs:comment "A structure to provide a URL link plus metadata associated with the link." .

untp-core:Location a rdfs:Class ;
  rdfs:label "Location" ;
  rdfs:comment "Location information including address and geo-location of points, areas, and boundaries" .

untp-core:Material a rdfs:Class ;
  rdfs:label "Material" ;
  rdfs:comment "The material class encapsulates details about the origin or source of raw materials in a product, including the country of origin and the mass fraction." .

untp-core:Measure a rdfs:Class ;
  rdfs:label "Measure" ;
  rdfs:comment "The measure class defines a numeric measured value (eg 10) and a coded unit of measure (eg KG)." .

untp-core:Metric a rdfs:Class ;
  rdfs:label "Metric" ;
  rdfs:comment "A specific measure of performance against the criteria that governs the claim.  Expressed as an array of metric (ie unit of measure) / value (ie the actual numeric value) pairs.  " .

untp-core:Party a rdfs:Class ;
  rdfs:label "Party" ;
  rdfs:comment "An organisation.  May be a supply chain actor, a certifier, a government agency." .

untp-core:Product a rdfs:Class ;
  rdfs:label "Product" ;
  rdfs:comment "The ProductInformation class encapsulates detailed information regarding a specific product, including its identification details, manufacturer, and other pertinent details." .

untp-core:Regulation a rdfs:Class ;
  rdfs:label "Regulation" ;
  rdfs:comment "A regulation (eg EU deforestation regulation) that defines the criteria for assessment." .

untp-core:RenderTemplate2024 a rdfs:Class ;
  rdfs:label "RenderTemplate2024" ;
  rdfs:comment "A single template format focused render method--where the content/media type decision becomes secondary (and is expressed separately).See https://github.com/w3c-ccg/vc-render-method/issues/9" .

untp-core:SecureLink a rdfs:Class ;
  rdfs:label "SecureLink" ;
  rdfs:comment "A binary file that is hashed ()for tamper evidence) and optionally encrypted (for confidentiality)." ;
  rdfs:subClassOf "untp-core:Link" .

untp-core:Standard a rdfs:Class ;
  rdfs:label "Standard" ;
  rdfs:comment "A standard (eg ISO 14000) that specifies the criteria for conformance." .

untp-core:VerifiableCredential a rdfs:Class ;
  rdfs:label "VerifiableCredential" ;
  rdfs:comment "A verifiable credential is a digital and verifiable version of everyday credentials such as certificates and licenses.  It conforms to the W3C Verifiable Credentials Data Model v2.0 (VCDM). " .

untp-core:WebRenderingTemplate2022 a rdfs:Class ;
  rdfs:label "WebRenderingTemplate2022" ;
  rdfs:comment "A simple (though non-standard) embedded template." .

#################### Enumerations (Nomenclatures)

untp-core:assessmentLevelCode a rdfs:Class ;
  rdfs:label "assessmentLevelCode" ;
  rdfs:comment "Type of authority endorsement of the assessment process" .

untp-core:assessorLevelCode a rdfs:Class ;
  rdfs:label "assessorLevelCode" ;
  rdfs:comment "Code that describes the level of independent assurance of the specific assessment" .

untp-core:attestationTypeCode a rdfs:Class ;
  rdfs:label "attestationTypeCode" ;
  rdfs:comment "A code for the type of the attestation credential" .

untp-core:conformityTopicCode a rdfs:Class ;
  rdfs:label "conformityTopicCode" ;
  rdfs:comment "A high level category scheme for product and facility conformity declarations (claims or attestations)" .

untp-core:countryCode a rdfs:Class ;
  rdfs:label "countryCode" ;
  rdfs:comment "Country code list." .

untp-core:encryptionMethodCode a rdfs:Class ;
  rdfs:label "encryptionMethodCode" ;
  rdfs:comment "Encryption method code list" .

untp-core:hashMethodCode a rdfs:Class ;
  rdfs:label "hashMethodCode" ;
  rdfs:comment "Hash method code list" .

untp-core:mimeType a rdfs:Class ;
  rdfs:label "mimeType" ;
  rdfs:comment "IANA multipart media encoding type " .

untp-core:operationalScopeCode a rdfs:Class ;
  rdfs:label "operationalScopeCode" ;
  rdfs:comment "Code list to indicate scope 3 emissions operational boundaries" .

untp-core:performanceLevelCode a rdfs:Class ;
  rdfs:label "performanceLevelCode" ;
  rdfs:comment "Coe list to indicate the performance level (eg A, B, C) at which this criterion is targeted." .

untp-core:statusCode a rdfs:Class ;
  rdfs:label "statusCode" ;
  rdfs:comment "" .

untp-core:tagCode a rdfs:Class ;
  rdfs:label "tagCode" ;
  rdfs:comment "A set of tags that can be used to classify or group criteria" .

untp-core:topicCode a rdfs:Class ;
  rdfs:label "topicCode" ;
  rdfs:comment "" .

untp-core:unitOfMeasure a rdfs:Class ;
  rdfs:label "unitOfMeasure" ;
  rdfs:comment "UNECE Recommendation 20 Unit of Measure codelist" .

#################### Properties

untp-core:accuracy a owl:DatatypeProperty, rdf:Property ;
  rdfs:label "accuracy" ;
  rdfs:comment "A percentage represented as a numeric between 0 and 1 indicating the rage of accuracy of the claimed value (eg 0.05 means that the actual value is within 5% of the claimed value.)" ;
  schema:domainIncludes untp-core:Metric ;
  schema:rangeIncludes xsd:double .

untp-core:address a owl:ObjectProperty, rdf:Property ;
  rdfs:label "address" ;
  rdfs:comment "The Postal address of the location." ;
  schema:domainIncludes untp-core:Facility ;
  schema:rangeIncludes untp-core:Address .

untp-core:addressCountry a owl:ObjectProperty, rdf:Property ;
  rdfs:label "addressCountry" ;
  rdfs:comment "The address country as an ISO-3166 two letter country code." ;
  schema:domainIncludes untp-core:Address ;
  schema:rangeIncludes untp-core:countryCode .

untp-core:addressLocality a owl:DatatypeProperty, rdf:Property ;
  rdfs:label "addressLocality" ;
  rdfs:comment "The city, suburb or township name." ;
  schema:domainIncludes untp-core:Address ;
  schema:rangeIncludes xsd:string .

untp-core:addressRegion a owl:DatatypeProperty, rdf:Property ;
  rdfs:label "addressRegion" ;
  rdfs:comment "The state or territory or province" ;
  schema:domainIncludes untp-core:Address ;
  schema:rangeIncludes xsd:string .

untp-core:administeredBy a owl:ObjectProperty, rdf:Property ;
  rdfs:label "administeredBy" ;
  rdfs:comment "the issuing body of the regulation. For example Australian Government Department of Climate Change, Energy, the Environment and Water" ;
  schema:domainIncludes untp-core:Regulation ;
  schema:rangeIncludes untp-core:Party .

untp-core:assessmentCriteria a owl:ObjectProperty, rdf:Property ;
  rdfs:label "assessmentCriteria" ;
  rdfs:comment "The specification against which the assessment is made." ;
  schema:domainIncludes untp-core:Claim, untp-core:Declaration ;
  schema:rangeIncludes untp-core:Criterion .

untp-core:assessmentDate a owl:DatatypeProperty, rdf:Property ;
  rdfs:label "assessmentDate" ;
  rdfs:comment "The date on which this assessment was made. " ;
  schema:domainIncludes untp-core:Claim, untp-core:Declaration ;
  schema:rangeIncludes xsd:string .

untp-core:assessmentLevel a owl:ObjectProperty, rdf:Property ;
  rdfs:label "assessmentLevel" ;
  rdfs:comment "Assurance pertaining to assessment (any authority or support for the assessment process)" ;
  schema:domainIncludes untp-core:Attestation ;
  schema:rangeIncludes untp-core:assessmentLevelCode .

untp-core:assessorLevel a owl:ObjectProperty, rdf:Property ;
  rdfs:label "assessorLevel" ;
  rdfs:comment "Assurance code pertaining to assessor (relation to the object under assessment)" ;
  schema:domainIncludes untp-core:Attestation ;
  schema:rangeIncludes untp-core:assessorLevelCode .

untp-core:attestationType a owl:ObjectProperty, rdf:Property ;
  rdfs:label "attestationType" ;
  rdfs:comment "The type of criterion (optional or mandatory)." ;
  schema:domainIncludes untp-core:Attestation ;
  schema:rangeIncludes untp-core:attestationTypeCode .

untp-core:auditableEvidence a owl:ObjectProperty, rdf:Property ;
  rdfs:label "auditableEvidence" ;
  rdfs:comment "Auditable evidence supporting this assessment such as raw measurements, supporting documents. This is usually private data and would normally be encrypted." ;
  schema:domainIncludes untp-core:Attestation ;
  schema:rangeIncludes untp-core:SecureLink .

untp-core:authorisation a owl:ObjectProperty, rdf:Property ;
  rdfs:label "authorisation" ;
  rdfs:comment "The authority under which a conformity claim is issued.  For example a national accreditation authority may authorise a test lab to issue test certificates about a product against a standard.  " ;
  schema:domainIncludes untp-core:Attestation ;
  schema:rangeIncludes untp-core:Endorsement .

untp-core:batchNumber a owl:DatatypeProperty, rdf:Property ;
  rdfs:label "batchNumber" ;
  rdfs:comment "Identifier of the specific production batch of the product.  Unique within the product class." ;
  schema:domainIncludes untp-core:Product ;
  schema:rangeIncludes xsd:string .

untp-core:carbonFootprint a owl:DatatypeProperty, rdf:Property ;
  rdfs:label "carbonFootprint" ;
  rdfs:comment "The carbon footprint of the product in KgCO2e per declared unit." ;
  schema:domainIncludes untp-core:EmissionsPerformance ;
  schema:rangeIncludes xsd:double .

untp-core:category a owl:ObjectProperty, rdf:Property ;
  rdfs:label "category" ;
  rdfs:comment "A set of classification codes that may be used to categorize the applicability of this criteria - for example industry sector, jurisdiction or commodity type - based on a formal vocabulary." ;
  schema:domainIncludes untp-core:Criterion ;
  schema:rangeIncludes untp-core:Classification .

untp-core:characteristics a owl:ObjectProperty, rdf:Property ;
  rdfs:label "characteristics" ;
  rdfs:comment "A placeholder for indusutry / product category specific information. " ;
  schema:domainIncludes untp-core:Product ;
  schema:rangeIncludes untp-core:Characteristics .

untp-core:code a owl:DatatypeProperty, rdf:Property ;
  rdfs:label "code" ;
  rdfs:comment "classification code within the scheme" ;
  schema:domainIncludes untp-core:Classification ;
  schema:rangeIncludes xsd:string .

untp-core:conformance a owl:DatatypeProperty, rdf:Property ;
  rdfs:label "conformance" ;
  rdfs:comment "An indicator of whether or not the claim or assesment conforms to the regulatory or standard criteria." ;
  schema:domainIncludes untp-core:Claim, untp-core:Declaration ;
  schema:rangeIncludes xsd:boolean .

untp-core:conformityCertificate a owl:ObjectProperty, rdf:Property ;
  rdfs:label "conformityCertificate" ;
  rdfs:comment "A reference to the human / printable version of this conformity attestation - typically represented as a PDF document. The document may have more details than are represented in the digital attestation." ;
  schema:domainIncludes untp-core:Attestation ;
  schema:rangeIncludes untp-core:SecureLink .

untp-core:conformityEvidence a owl:ObjectProperty, rdf:Property ;
  rdfs:label "conformityEvidence" ;
  rdfs:comment "A URI pointing to the evidence supporting the claim. SHOULD be a URL to a UNTP Digital Conformity Credential (DCC)" ;
  schema:domainIncludes untp-core:Claim ;
  schema:rangeIncludes untp-core:SecureLink .

untp-core:conformityTopic a owl:ObjectProperty, rdf:Property ;
  rdfs:label "conformityTopic" ;
  rdfs:comment "A gloabl UN/CEFACT standard sustainability toipic code. ", "The conformity topic category for this assessment (eg vocabulary.uncefact.org/sustainability/emissions)" ;
  schema:domainIncludes untp-core:Claim, untp-core:Criterion, untp-core:Declaration ;
  schema:rangeIncludes untp-core:conformityTopicCode .

untp-core:countryOfOperation a owl:ObjectProperty, rdf:Property ;
  rdfs:label "countryOfOperation" ;
  rdfs:comment "The country in which this facility is operating." ;
  schema:domainIncludes untp-core:Facility ;
  schema:rangeIncludes untp-core:countryCode .

untp-core:countryOfProduction a owl:ObjectProperty, rdf:Property ;
  rdfs:label "countryOfProduction" ;
  rdfs:comment "The country in which this item was produced / manufactured." ;
  schema:domainIncludes untp-core:Product ;
  schema:rangeIncludes untp-core:countryCode .

untp-core:declaredUnit a owl:ObjectProperty, rdf:Property ;
  rdfs:label "declaredUnit" ;
  rdfs:comment "The unit of product (EA, KGM, LTR, etc) that is the basis for carbon footprint." ;
  schema:domainIncludes untp-core:EmissionsPerformance ;
  schema:rangeIncludes untp-core:unitOfMeasure .

untp-core:declaredValue a owl:ObjectProperty, rdf:Property ;
  rdfs:label "declaredValue" ;
  rdfs:comment "The list of specific values measured as part of this assessment (eg tensile strength)" ;
  schema:domainIncludes untp-core:Claim, untp-core:Declaration ;
  schema:rangeIncludes untp-core:Metric .

untp-core:description a owl:DatatypeProperty, rdf:Property ;
  rdfs:label "description" ;
  rdfs:comment "A full text description of the criterion that clearly specifies how compliance is achieved and measured. ", "A textual description of the declaration being made.", "A textual description of the scope or purpose of this conformity attestation", "A textual description providing details about the product.", "An optional short description of the facility", "An optional short description of the party.", "The description of this conformity scheme" ;
  schema:domainIncludes untp-core:Attestation, untp-core:Claim, untp-core:ConformityScheme, untp-core:Criterion, untp-core:Declaration, untp-core:Facility, untp-core:Party, untp-core:Product ;
  schema:rangeIncludes xsd:string .

untp-core:digestMultibase a owl:DatatypeProperty, rdf:Property ;
  rdfs:label "digestMultibase" ;
  rdfs:comment "Used for resource integrity and/or validation of the inline `template`" ;
  schema:domainIncludes untp-core:RenderTemplate2024 ;
  schema:rangeIncludes xsd:string .

untp-core:dimensions a owl:ObjectProperty, rdf:Property ;
  rdfs:label "dimensions" ;
  rdfs:comment "The physical dimensions of the product. Not every dimension is relevant to every products.  For example bulk materials may have weight and volume but not length, with, or height.\"weight\":{\"value\":10, \"unit\":\"KGM\"}" ;
  schema:domainIncludes untp-core:Product ;
  schema:rangeIncludes untp-core:Dimension .

untp-core:effectiveDate a owl:DatatypeProperty, rdf:Property ;
  rdfs:label "effectiveDate" ;
  rdfs:comment "the date at which the regulation came into effect." ;
  schema:domainIncludes untp-core:Regulation ;
  schema:rangeIncludes xsd:string .

untp-core:encryptionMethod a owl:ObjectProperty, rdf:Property ;
  rdfs:label "encryptionMethod" ;
  rdfs:comment "The symmetric encryption algorithm used to encrypt the link target.  AES is the recommended standard. Decryption keys are expected to be passed out of bounds." ;
  schema:domainIncludes untp-core:SecureLink ;
  schema:rangeIncludes untp-core:encryptionMethodCode .

untp-core:endorsementEvidence a owl:ObjectProperty, rdf:Property ;
  rdfs:label "endorsementEvidence" ;
  rdfs:comment "The evidence that supports the authority under which the attestation is issued - for an example an accreditation certificate." ;
  schema:domainIncludes untp-core:Endorsement ;
  schema:rangeIncludes untp-core:Link .

untp-core:facilityAlsoKnownAs a owl:ObjectProperty, rdf:Property ;
  rdfs:label "facilityAlsoKnownAs" ;
  rdfs:comment "An optional list of other registered identifiers for this facility - eg GLNs or other schemes." ;
  schema:domainIncludes untp-core:Facility ;
  schema:rangeIncludes untp-core:Facility .

untp-core:file a owl:DatatypeProperty, rdf:Property ;
  rdfs:label "file" ;
  rdfs:comment "The binary file data encoded as Base64 string." ;
  schema:domainIncludes untp-core:BinaryFile ;
  schema:rangeIncludes xsd:string .

untp-core:fileName a owl:DatatypeProperty, rdf:Property ;
  rdfs:label "fileName" ;
  rdfs:comment "A name for referenced binary file" ;
  schema:domainIncludes untp-core:BinaryFile ;
  schema:rangeIncludes xsd:string .

untp-core:fileType a owl:ObjectProperty, rdf:Property ;
  rdfs:label "fileType" ;
  rdfs:comment "The type of file, represented as a MIME type." ;
  schema:domainIncludes untp-core:BinaryFile ;
  schema:rangeIncludes untp-core:mimeType .

untp-core:furtherInformation a owl:ObjectProperty, rdf:Property ;
  rdfs:label "furtherInformation" ;
  rdfs:comment "A URL pointing to further human readable information about the product." ;
  schema:domainIncludes untp-core:Product ;
  schema:rangeIncludes untp-core:Link .

untp-core:geoBoundary a owl:ObjectProperty, rdf:Property ;
  rdfs:label "geoBoundary" ;
  rdfs:comment "The list of ordered coordinates that define a closed area polygon as a location boundary using GeoJSON polygon notation." ;
  schema:domainIncludes untp-core:Location ;
  schema:rangeIncludes geojson:appendix-A.3 .

untp-core:geoLocation a owl:ObjectProperty, rdf:Property ;
  rdfs:label "geoLocation" ;
  rdfs:comment "The latitude and longitude coordinates that best represent the specified location. Using GeoJSON Point notation." ;
  schema:domainIncludes untp-core:Location ;
  schema:rangeIncludes geojson:appendix-A.1 .

untp-core:hashDigest a owl:DatatypeProperty, rdf:Property ;
  rdfs:label "hashDigest" ;
  rdfs:comment "The hash of the file." ;
  schema:domainIncludes untp-core:SecureLink ;
  schema:rangeIncludes xsd:string .

untp-core:hashMethod a owl:ObjectProperty, rdf:Property ;
  rdfs:label "hashMethod" ;
  rdfs:comment "The hashing algorithm used to create the target hash.  SHA-265 is the recommended standard" ;
  schema:domainIncludes untp-core:SecureLink ;
  schema:rangeIncludes untp-core:hashMethodCode .

untp-core:hazardous a owl:DatatypeProperty, rdf:Property ;
  rdfs:label "hazardous" ;
  rdfs:comment "Indicates whether this material is hazardous. If true then the materialSafetyInformation property must be present" ;
  schema:domainIncludes untp-core:Material ;
  schema:rangeIncludes xsd:boolean .

untp-core:height a owl:ObjectProperty, rdf:Property ;
  rdfs:label "height" ;
  rdfs:comment "The height of the product or packaging. eg {\"value\":220, \"unit\":\"MMT\"}" ;
  schema:domainIncludes untp-core:Dimension ;
  schema:rangeIncludes untp-core:Measure .

untp-core:id a owl:DatatypeProperty, rdf:Property ;
  rdfs:label "id" ;
  rdfs:comment "A unique identifier for the criterion within the scheme, standard  or regulation. For example CO2 emissions calculations for liquid fuel combustion.", "A unique identifier for the declaration. Often this will be an extension of the product.id or attestation.id. But could be a UUID.", "A unique identifier for the standard (eg https://www.iso.org/standard/60857.html).", "Globally unique identifier of an accreditation or authority issued to a conformity assessment body by a regulator or national accreditation authority.", "The W3C DID of the issuer - should be a did:web or did:webvh", "The globally unique ID of the facility as URI, ideally as a resolvable URL.", "The globally unique ID of the party as a URI, ideally as a resolvable ID. ", "The globally unique ID of the product as a URI. Ideally as a resolvable URL according to ISO 18975. ", "The globally unique ID of this conformity attestation.", "The globally unique URI representing the specific classifier value", "The globally unique identifier of the registration scheme. The scheme should be registered and discoverable from vocabulary.uncefact.org/identifierSchemes", "The globally unique identifier of this regulation. ", "The identifier of this scheme as a URI. Typically of the form ownerDomain.schemeName." ;
  schema:domainIncludes untp-core:Attestation, untp-core:Claim, untp-core:Classification, untp-core:ConformityScheme, untp-core:CredentialIssuer, untp-core:Criterion, untp-core:Declaration, untp-core:Endorsement, untp-core:Facility, untp-core:IdentifierScheme, untp-core:Party, untp-core:Product, untp-core:Regulation, untp-core:Standard ;
  schema:rangeIncludes xsd:string .

untp-core:idScheme a owl:ObjectProperty, rdf:Property ;
  rdfs:label "idScheme" ;
  rdfs:comment "The ID scheme of the facility. eg a GS1 GLN or a National land registry scheme. If self issued then use the party ID of the facility owner. ", "The identifier scheme for this product.  Eg a GS1 GTIN or an AU Livestock NLIS, or similar. If self issued then use the party ID of the issuer.  ", "The identifier scheme of the party.  Typically a national business register or a global scheme such as GLEIF. " ;
  schema:domainIncludes untp-core:Facility, untp-core:Party, untp-core:Product ;
  schema:rangeIncludes untp-core:IdentifierScheme .

untp-core:industryCategory a owl:ObjectProperty, rdf:Property ;
  rdfs:label "industryCategory" ;
  rdfs:comment "The industry categories for this organisations.  Recommend use of UNCPC as the category scheme. for example - unstats.un.org/isic/1030" ;
  schema:domainIncludes untp-core:Party ;
  schema:rangeIncludes untp-core:Classification .

untp-core:issueDate a owl:DatatypeProperty, rdf:Property ;
  rdfs:label "issueDate" ;
  rdfs:comment "The date when the standard was issued." ;
  schema:domainIncludes untp-core:Standard ;
  schema:rangeIncludes xsd:string .

untp-core:issuedToParty a owl:ObjectProperty, rdf:Property ;
  rdfs:label "issuedToParty" ;
  rdfs:comment "The party to whom the conformity attestation was issued." ;
  schema:domainIncludes untp-core:Attestation ;
  schema:rangeIncludes untp-core:Party .

untp-core:issuerAlsoKnownAs a owl:ObjectProperty, rdf:Property ;
  rdfs:label "issuerAlsoKnownAs" ;
  rdfs:comment "An optional list of other registered identifiers for this credential issuer " ;
  schema:domainIncludes untp-core:CredentialIssuer ;
  schema:rangeIncludes untp-core:Party .

untp-core:issuingAuthority a owl:ObjectProperty, rdf:Property ;
  rdfs:label "issuingAuthority" ;
  rdfs:comment "The competent authority that issued the accreditation." ;
  schema:domainIncludes untp-core:Endorsement ;
  schema:rangeIncludes untp-core:Party .

untp-core:issuingParty a owl:ObjectProperty, rdf:Property ;
  rdfs:label "issuingParty" ;
  rdfs:comment "The party that issued the standard " ;
  schema:domainIncludes untp-core:Standard ;
  schema:rangeIncludes untp-core:Party .

untp-core:jurisdictionCountry a owl:ObjectProperty, rdf:Property ;
  rdfs:label "jurisdictionCountry" ;
  rdfs:comment "The legal jurisdiction (country) under which the regulation is issued." ;
  schema:domainIncludes untp-core:Regulation ;
  schema:rangeIncludes untp-core:countryCode .

untp-core:length a owl:ObjectProperty, rdf:Property ;
  rdfs:label "length" ;
  rdfs:comment "The length of the product or packaging eg {\"value\":840, \"unit\":\"MMT\"}" ;
  schema:domainIncludes untp-core:Dimension ;
  schema:rangeIncludes untp-core:Measure .

untp-core:linkName a owl:DatatypeProperty, rdf:Property ;
  rdfs:label "linkName" ;
  rdfs:comment "A display name for the target resource " ;
  schema:domainIncludes untp-core:Link, untp-core:SecureLink ;
  schema:rangeIncludes xsd:string .

untp-core:linkType a owl:DatatypeProperty, rdf:Property ;
  rdfs:label "linkType" ;
  rdfs:comment "The type of the target resource - drawn from a controlled vocabulary " ;
  schema:domainIncludes untp-core:Link, untp-core:SecureLink ;
  schema:rangeIncludes xsd:string .

untp-core:linkURL a owl:DatatypeProperty, rdf:Property ;
  rdfs:label "linkURL" ;
  rdfs:comment "The URL of the target resource. " ;
  schema:domainIncludes untp-core:Link, untp-core:SecureLink ;
  schema:rangeIncludes xsd:string .

untp-core:locationInformation a owl:ObjectProperty, rdf:Property ;
  rdfs:label "locationInformation" ;
  rdfs:comment "Geo-location information for this facility as a resolvable geographic area (a Plus Code), and/or a geo-located point (latitude / longitude), and/or a defined boundary (GeoJSON Polygon)." ;
  schema:domainIncludes untp-core:Facility ;
  schema:rangeIncludes untp-core:Location .

untp-core:mass a owl:ObjectProperty, rdf:Property ;
  rdfs:label "mass" ;
  rdfs:comment "The mass of the material component." ;
  schema:domainIncludes untp-core:Material ;
  schema:rangeIncludes untp-core:Measure .

untp-core:massFraction a owl:DatatypeProperty, rdf:Property ;
  rdfs:label "massFraction" ;
  rdfs:comment "The mass fraction of the product represented by this material. The sum of all mass fraction values for a given passport should be 1." ;
  schema:domainIncludes untp-core:Material ;
  schema:rangeIncludes xsd:double .

untp-core:materialCircularityIndicator a owl:DatatypeProperty, rdf:Property ;
  rdfs:label "materialCircularityIndicator" ;
  rdfs:comment "The overall circularity performance indicator for this product. Calculated as 1 - (V+W)/2D where - V = Virgin material proportion by mass (will be 1- recycled content) - W = Waste leakage proportion by mass (will be 1 - recyclableContent)  - D = Utility factor (set to 1 if unknown).  " ;
  schema:domainIncludes untp-core:CircularityPerformance ;
  schema:rangeIncludes xsd:double .

untp-core:materialSafetyInformation a owl:ObjectProperty, rdf:Property ;
  rdfs:label "materialSafetyInformation" ;
  rdfs:comment "Reference to further information about safe handling of this hazardous material (for example a link to a material safety data sheet)" ;
  schema:domainIncludes untp-core:Material ;
  schema:rangeIncludes untp-core:Link .

untp-core:materialType a owl:ObjectProperty, rdf:Property ;
  rdfs:label "materialType" ;
  rdfs:comment "The type of this material - as a value drawn from a controlled vocabulary eg from UN Framework Classification for Resources (UNFC)." ;
  schema:domainIncludes untp-core:Material ;
  schema:rangeIncludes untp-core:Classification .

untp-core:mediaQuery a owl:DatatypeProperty, rdf:Property ;
  rdfs:label "mediaQuery" ;
  rdfs:comment "Media query as defined in https://www.w3.org/TR/mediaqueries-4/" ;
  schema:domainIncludes untp-core:RenderTemplate2024 ;
  schema:rangeIncludes xsd:string .

untp-core:mediaType a owl:DatatypeProperty, rdf:Property ;
  rdfs:label "mediaType" ;
  rdfs:comment "content/media type for (possible) conneg on the above URL and certainly for display use" ;
  schema:domainIncludes untp-core:RenderTemplate2024 ;
  schema:rangeIncludes xsd:string .

untp-core:metricName a owl:DatatypeProperty, rdf:Property ;
  rdfs:label "metricName" ;
  rdfs:comment "A human readable name for this metric (for example \"Tensile strength\")" ;
  schema:domainIncludes untp-core:Metric ;
  schema:rangeIncludes xsd:string .

untp-core:metricValue a owl:ObjectProperty, rdf:Property ;
  rdfs:label "metricValue" ;
  rdfs:comment "A numeric value and unit of measure for this metric. Could be a measured value or a specified threshold. Eg {\"value\":400, \"unit\":\"MPA\"} as tensile strength of structural steel" ;
  schema:domainIncludes untp-core:Metric ;
  schema:rangeIncludes untp-core:Measure .

untp-core:name a owl:DatatypeProperty, rdf:Property ;
  rdfs:label "name" ;
  rdfs:comment "A human readable description of this conformity attestation", "A name that describes this criteria.", "Human facing display name for selection", "Human facing display name for template", "Name of the classification represented by the code", "Name of this material (eg \"Egyptian Cotton\")", "The name of the accreditation.", "The name of the identifier scheme. ", "The name of the issuer person or organisation", "The name of the regulation or act.", "The name of the standard", "The name of this conformity scheme", "The registered name of the facility within the identifier scheme.  ", "The registered name of the party within the identifier scheme.", "The registered name of the product within the identifier scheme. " ;
  schema:domainIncludes untp-core:Attestation, untp-core:Classification, untp-core:ConformityScheme, untp-core:CredentialIssuer, untp-core:Criterion, untp-core:Endorsement, untp-core:Facility, untp-core:IdentifierScheme, untp-core:Material, untp-core:Party, untp-core:Product, untp-core:Regulation, untp-core:RenderTemplate2024, untp-core:Standard, untp-core:WebRenderingTemplate2022 ;
  schema:rangeIncludes xsd:string .

untp-core:operatedByParty a owl:ObjectProperty, rdf:Property ;
  rdfs:label "operatedByParty" ;
  rdfs:comment "The Party entity responsible for operating the facility.An object structure that uniquely identifies the party within a known party identification scheme. " ;
  schema:domainIncludes untp-core:Facility ;
  schema:rangeIncludes untp-core:Party .

untp-core:operationalScope a owl:ObjectProperty, rdf:Property ;
  rdfs:label "operationalScope" ;
  rdfs:comment "The operational scope of the emissions performance. Only scope 1 & 2, or including upstream scope 3 (cradle to gate) or upstream and downstream scope 3 (cradle to grave)." ;
  schema:domainIncludes untp-core:EmissionsPerformance ;
  schema:rangeIncludes untp-core:operationalScopeCode .

untp-core:organisationWebsite a owl:DatatypeProperty, rdf:Property ;
  rdfs:label "organisationWebsite" ;
  rdfs:comment "Website for this organisation" ;
  schema:domainIncludes untp-core:Party ;
  schema:rangeIncludes xsd:string .

untp-core:originCountry a owl:ObjectProperty, rdf:Property ;
  rdfs:label "originCountry" ;
  rdfs:comment "A ISO 3166-1 code representing the country of origin of the component or ingredient." ;
  schema:domainIncludes untp-core:Material ;
  schema:rangeIncludes untp-core:countryCode .

untp-core:owner a owl:ObjectProperty, rdf:Property ;
  rdfs:label "owner" ;
  rdfs:comment "The party that is the owner / maintainer of this conformity scheme." ;
  schema:domainIncludes untp-core:ConformityScheme ;
  schema:rangeIncludes untp-core:Party .

untp-core:partyAlsoKnownAs a owl:ObjectProperty, rdf:Property ;
  rdfs:label "partyAlsoKnownAs" ;
  rdfs:comment "An optional list of other registered identifiers for this organisation. For example DUNS, GLN, LEI, etc" ;
  schema:domainIncludes untp-core:Party ;
  schema:rangeIncludes untp-core:Party .

untp-core:performanceLevel a owl:DatatypeProperty, rdf:Property ;
  rdfs:label "performanceLevel" ;
  rdfs:comment "A performance category code to group criterion in a given hierarchyLevel according to pareformance" ;
  schema:domainIncludes untp-core:Criterion ;
  schema:rangeIncludes xsd:string .

untp-core:plusCode a owl:DatatypeProperty, rdf:Property ;
  rdfs:label "plusCode" ;
  rdfs:comment "An open location code (https://maps.google.com/pluscodes/) representing this geographic location or region. Open location codes can represent any sized area from a point to a large region and are easily resolved to a visual map location. " ;
  schema:domainIncludes untp-core:Location ;
  schema:rangeIncludes xsd:string .

untp-core:postalCode a owl:DatatypeProperty, rdf:Property ;
  rdfs:label "postalCode" ;
  rdfs:comment "The postal code or zip code for this address." ;
  schema:domainIncludes untp-core:Address ;
  schema:rangeIncludes xsd:string .

untp-core:primarySourcedRatio a owl:DatatypeProperty, rdf:Property ;
  rdfs:label "primarySourcedRatio" ;
  rdfs:comment "The ratio of emissions data from primary sources (ie from supplier / product specific information rather than secondary / industry averages)." ;
  schema:domainIncludes untp-core:EmissionsPerformance ;
  schema:rangeIncludes xsd:double .

untp-core:processCategory a owl:ObjectProperty, rdf:Property ;
  rdfs:label "processCategory" ;
  rdfs:comment "The industrial or production processes performed by this facility. Example unstats.un.org/isic/1030." ;
  schema:domainIncludes untp-core:Facility ;
  schema:rangeIncludes untp-core:Classification .

untp-core:producedAtFacility a owl:ObjectProperty, rdf:Property ;
  rdfs:label "producedAtFacility" ;
  rdfs:comment "The Facility where the product batch was produced / manufactured." ;
  schema:domainIncludes untp-core:Product ;
  schema:rangeIncludes untp-core:Facility .

untp-core:producedByParty a owl:ObjectProperty, rdf:Property ;
  rdfs:label "producedByParty" ;
  rdfs:comment "The Party entity that manufactured the product." ;
  schema:domainIncludes untp-core:Product ;
  schema:rangeIncludes untp-core:Party .

untp-core:productCategory a owl:ObjectProperty, rdf:Property ;
  rdfs:label "productCategory" ;
  rdfs:comment "A code representing the product's class, typically using the UN CPC (United Nations Central Product Classification) https://unstats.un.org/unsd/classifications/Econ/cpc" ;
  schema:domainIncludes untp-core:Product ;
  schema:rangeIncludes untp-core:Classification .

untp-core:productImage a owl:ObjectProperty, rdf:Property ;
  rdfs:label "productImage" ;
  rdfs:comment "Reference information (location, type, name) of an image of the product." ;
  schema:domainIncludes untp-core:Product ;
  schema:rangeIncludes untp-core:Link .

untp-core:productionDate a owl:DatatypeProperty, rdf:Property ;
  rdfs:label "productionDate" ;
  rdfs:comment "The ISO 8601 date on which the product batch or individual serialised item was manufactured." ;
  schema:domainIncludes untp-core:Product ;
  schema:rangeIncludes xsd:string .

untp-core:recyclableContent a owl:DatatypeProperty, rdf:Property ;
  rdfs:label "recyclableContent" ;
  rdfs:comment "The fraction of the this product (my mass) that has been designed to be recyclable / re-usable. This will be be the total fraction that can avoid waste / landfill." ;
  schema:domainIncludes untp-core:CircularityPerformance ;
  schema:rangeIncludes xsd:double .

untp-core:recycledContent a owl:DatatypeProperty, rdf:Property ;
  rdfs:label "recycledContent" ;
  rdfs:comment "The fraction (by mass) of recycled / repurposed, repaired content in this product.  This will be the total virgin content fraction." ;
  schema:domainIncludes untp-core:CircularityPerformance ;
  schema:rangeIncludes xsd:double .

untp-core:recycledMassFraction a owl:DatatypeProperty, rdf:Property ;
  rdfs:label "recycledMassFraction" ;
  rdfs:comment "Mass fraction of this material that is recycled (eg 50% recycled Lithium)" ;
  schema:domainIncludes untp-core:Material ;
  schema:rangeIncludes xsd:double .

untp-core:recyclingInformation a owl:ObjectProperty, rdf:Property ;
  rdfs:label "recyclingInformation" ;
  rdfs:comment "A URI pointing to recycling information for the product." ;
  schema:domainIncludes untp-core:CircularityPerformance ;
  schema:rangeIncludes untp-core:Link .

untp-core:referenceRegulation a owl:ObjectProperty, rdf:Property ;
  rdfs:label "referenceRegulation" ;
  rdfs:comment "The reference to the regulation that defines the assessment criteria" ;
  schema:domainIncludes untp-core:Claim, untp-core:Declaration ;
  schema:rangeIncludes untp-core:Regulation .

untp-core:referenceStandard a owl:ObjectProperty, rdf:Property ;
  rdfs:label "referenceStandard" ;
  rdfs:comment "The reference to the standard that defines the specification / criteria" ;
  schema:domainIncludes untp-core:Claim, untp-core:Declaration ;
  schema:rangeIncludes untp-core:Standard .

untp-core:registeredId a owl:DatatypeProperty, rdf:Property ;
  rdfs:label "registeredId" ;
  rdfs:comment "The registration number (alphanumeric) of the Party within the register. Unique within the register.", "The registration number (alphanumeric) of the entity within the register. Unique within the register.", "The registration number (alphanumeric) of the facility within the identifier scheme. Unique within the register." ;
  schema:domainIncludes untp-core:Facility, untp-core:Party, untp-core:Product ;
  schema:rangeIncludes xsd:string .

untp-core:registrationCountry a owl:ObjectProperty, rdf:Property ;
  rdfs:label "registrationCountry" ;
  rdfs:comment "the country in which this organisation is registered" ;
  schema:domainIncludes untp-core:Party ;
  schema:rangeIncludes untp-core:countryCode .

untp-core:repairInformation a owl:ObjectProperty, rdf:Property ;
  rdfs:label "repairInformation" ;
  rdfs:comment "A URI pointing to repair instructions for this product." ;
  schema:domainIncludes untp-core:CircularityPerformance ;
  schema:rangeIncludes untp-core:Link .

untp-core:reportingStandard a owl:ObjectProperty, rdf:Property ;
  rdfs:label "reportingStandard" ;
  rdfs:comment "The reporting standard (eg GHG Protocol, IFRS S2, ESRS, etc) against which this product emissions performance is assessed." ;
  schema:domainIncludes untp-core:EmissionsPerformance ;
  schema:rangeIncludes untp-core:Standard .

untp-core:schemeID a owl:DatatypeProperty, rdf:Property ;
  rdfs:label "schemeID" ;
  rdfs:comment "Classification scheme ID" ;
  schema:domainIncludes untp-core:Classification ;
  schema:rangeIncludes xsd:string .

untp-core:schemeName a owl:DatatypeProperty, rdf:Property ;
  rdfs:label "schemeName" ;
  rdfs:comment "The name of the classification scheme" ;
  schema:domainIncludes untp-core:Classification ;
  schema:rangeIncludes xsd:string .

untp-core:score a owl:DatatypeProperty, rdf:Property ;
  rdfs:label "score" ;
  rdfs:comment "A score or rank associated with this measured metric." ;
  schema:domainIncludes untp-core:Metric ;
  schema:rangeIncludes xsd:string .

untp-core:serialNumber a owl:DatatypeProperty, rdf:Property ;
  rdfs:label "serialNumber" ;
  rdfs:comment "A number or code representing a specific serialised item of the product. Unique within product class." ;
  schema:domainIncludes untp-core:Product ;
  schema:rangeIncludes xsd:string .

untp-core:status a owl:ObjectProperty, rdf:Property ;
  rdfs:label "status" ;
  rdfs:comment "The lifecycle status of this criterion. " ;
  schema:domainIncludes untp-core:Criterion ;
  schema:rangeIncludes untp-core:statusCode .

untp-core:streetAddress a owl:DatatypeProperty, rdf:Property ;
  rdfs:label "streetAddress" ;
  rdfs:comment "the street address as an unstructured string." ;
  schema:domainIncludes untp-core:Address ;
  schema:rangeIncludes xsd:string .

untp-core:subCriterion a owl:ObjectProperty, rdf:Property ;
  rdfs:label "subCriterion" ;
  rdfs:comment "List of criterion that are subordinate to this criterion in the hierarchy." ;
  schema:domainIncludes untp-core:Criterion ;
  schema:rangeIncludes untp-core:Criterion .

untp-core:symbol a owl:DatatypeProperty, rdf:Property ;
  rdfs:label "symbol" ;
  rdfs:comment "Based 64 encoded binary used to represent a visual symbol for a given material. " ;
  schema:domainIncludes untp-core:Material ;
  schema:rangeIncludes xsd:string .

untp-core:tag a owl:DatatypeProperty, rdf:Property ;
  rdfs:label "tag" ;
  rdfs:comment "A set of tags that can be used by the scheme owner to be able to filter or group criterion in a large vocabulary for specific use cases." ;
  schema:domainIncludes untp-core:Criterion ;
  schema:rangeIncludes xsd:string .

untp-core:template a owl:DatatypeProperty, rdf:Property ;
  rdfs:label "template" ;
  rdfs:comment "An inline template field ", "An inline template field for use cases where remote retrieval of a render method is suboptimal" ;
  schema:domainIncludes untp-core:RenderTemplate2024, untp-core:WebRenderingTemplate2022 ;
  schema:rangeIncludes xsd:string .

untp-core:thresholdValue a owl:ObjectProperty, rdf:Property ;
  rdfs:label "thresholdValue" ;
  rdfs:comment "A threshold value that defines the minimum compliance level. " ;
  schema:domainIncludes untp-core:Criterion ;
  schema:rangeIncludes untp-core:Metric .

untp-core:trustmark a owl:ObjectProperty, rdf:Property ;
  rdfs:label "trustmark" ;
  rdfs:comment "The trust mark image awarded by the AB to the CAB to indicate accreditation.", "The trust mark or seal used by this conformity scheme." ;
  schema:domainIncludes untp-core:ConformityScheme, untp-core:Endorsement ;
  schema:rangeIncludes untp-core:BinaryFile .

untp-core:unit a owl:ObjectProperty, rdf:Property ;
  rdfs:label "unit" ;
  rdfs:comment "Unit of measure drawn from the UNECE Rec20 measure code list." ;
  schema:domainIncludes untp-core:Measure ;
  schema:rangeIncludes untp-core:unitOfMeasure .

untp-core:url a owl:DatatypeProperty, rdf:Property ;
  rdfs:label "url" ;
  rdfs:comment "URL for remotely hosted template" ;
  schema:domainIncludes untp-core:RenderTemplate2024 ;
  schema:rangeIncludes xsd:string .

untp-core:utilityFactor a owl:DatatypeProperty, rdf:Property ;
  rdfs:label "utilityFactor" ;
  rdfs:comment "An indicator of durability defined as the lifetime (typically measures as usage cycles) for this product divided by the industry average. For example a battery with a 10,000 cycle lifetime where industry average is 5,000 cycles will have a durability factor of 2. If unknown set to 1 or omit.  " ;
  schema:domainIncludes untp-core:CircularityPerformance ;
  schema:rangeIncludes xsd:double .

untp-core:validFrom a owl:DatatypeProperty, rdf:Property ;
  rdfs:label "validFrom" ;
  rdfs:comment "The data from which this scheme version is valid." ;
  schema:domainIncludes untp-core:ConformityScheme ;
  schema:rangeIncludes xsd:string .

untp-core:value a owl:DatatypeProperty, rdf:Property ;
  rdfs:label "value" ;
  rdfs:comment "The numeric value of the measure" ;
  schema:domainIncludes untp-core:Measure ;
  schema:rangeIncludes xsd:double .

untp-core:version a owl:DatatypeProperty, rdf:Property ;
  rdfs:label "version" ;
  rdfs:comment "Version of this scheme folling SemVer best practive (major.minor.patch). " ;
  schema:domainIncludes untp-core:ConformityScheme ;
  schema:rangeIncludes xsd:string .

untp-core:volume a owl:ObjectProperty, rdf:Property ;
  rdfs:label "volume" ;
  rdfs:comment "The displacement volume of the product. eg {\"value\":7.5, \"unit\":\"LTR\"}" ;
  schema:domainIncludes untp-core:Dimension ;
  schema:rangeIncludes untp-core:Measure .

untp-core:weight a owl:ObjectProperty, rdf:Property ;
  rdfs:label "weight" ;
  rdfs:comment "the weight of the product. EG {\"value\":10, \"unit\":\"KGM\"}" ;
  schema:domainIncludes untp-core:Dimension ;
  schema:rangeIncludes untp-core:Measure .

untp-core:width a owl:ObjectProperty, rdf:Property ;
  rdfs:label "width" ;
  rdfs:comment "The width of the product or packaging. eg {\"value\":150, \"unit\":\"MMT\"}" ;
  schema:domainIncludes untp-core:Dimension ;
  schema:rangeIncludes untp-core:Measure .

#################### Enumeration Values

<https://test.uncefact.org/vocabulary/untp/core/0/assessmentLevelCode#Accredited> a untp-core:assessmentLevelCode ;
  rdfs:label "National accreditation" ;
  rdfs:comment "conformity assessment delivered under an independent accreditation" ;
  rdf:value "Accredited" .

<https://test.uncefact.org/vocabulary/untp/core/0/assessmentLevelCode#GlobalMRA> a untp-core:assessmentLevelCode ;
  rdfs:label "Global mutual recognition agreement" ;
  rdfs:comment "conformity assessment delivered under authority granted by IAF/ILAC signatory body" ;
  rdf:value "GlobalMRA" .

<https://test.uncefact.org/vocabulary/untp/core/0/assessmentLevelCode#GovtApproval> a untp-core:assessmentLevelCode ;
  rdfs:label "Government endorsement" ;
  rdfs:comment "conformity assessment delivered under authority granted by national government" ;
  rdf:value "GovtApproval" .

<https://test.uncefact.org/vocabulary/untp/core/0/assessmentLevelCode#Unspecified> a untp-core:assessmentLevelCode ;
  rdfs:label "No endorsement." ;
  rdfs:comment "conformity assessment claiming no external authority or else unspecified" ;
  rdf:value "Unspecified" .

<https://test.uncefact.org/vocabulary/untp/core/0/assessmentLevelCode#Validated> a untp-core:assessmentLevelCode ;
  rdfs:label "External validation" ;
  rdfs:comment "conformity assessment externally validated" ;
  rdf:value "Validated" .

<https://test.uncefact.org/vocabulary/untp/core/0/assessmentLevelCode#Verified> a untp-core:assessmentLevelCode ;
  rdfs:label "External verification" ;
  rdfs:comment "conformity assessment externally verified" ;
  rdf:value "Verified" .

<https://test.uncefact.org/vocabulary/untp/core/0/assessorLevelCode#3rdParty> a untp-core:assessorLevelCode ;
  rdfs:label "Independent third party assessment" ;
  rdfs:comment " 3rd party (independent) conformity assessment" ;
  rdf:value "3rdParty" .

<https://test.uncefact.org/vocabulary/untp/core/0/assessorLevelCode#Buyer> a untp-core:assessorLevelCode ;
  rdfs:label "Buyer assessment" ;
  rdfs:comment " conformity assessment by potential purchaser" ;
  rdf:value "Buyer" .

<https://test.uncefact.org/vocabulary/untp/core/0/assessorLevelCode#Commercial> a untp-core:assessorLevelCode ;
  rdfs:label "Commercial assessment" ;
  rdfs:comment " conformity assessment by related body or under commercial contract" ;
  rdf:value "Commercial" .

<https://test.uncefact.org/vocabulary/untp/core/0/assessorLevelCode#Membership> a untp-core:assessorLevelCode ;
  rdfs:label "Industry body assessment" ;
  rdfs:comment " conformity assessment by industry representative body or membership body" ;
  rdf:value "Membership" .

<https://test.uncefact.org/vocabulary/untp/core/0/assessorLevelCode#Self> a untp-core:assessorLevelCode ;
  rdfs:label "Self assessed" ;
  rdfs:comment " self-assessment" ;
  rdf:value "Self" .

<https://test.uncefact.org/vocabulary/untp/core/0/assessorLevelCode#Unspecified> a untp-core:assessorLevelCode ;
  rdfs:label "No independent assessment" ;
  rdfs:comment " conformity assessment by party with unspecified relationship " ;
  rdf:value "Unspecified" .

<https://test.uncefact.org/vocabulary/untp/core/0/attestationTypeCode#calibration> a untp-core:attestationTypeCode ;
  rdfs:label "calibration" ;
  rdfs:comment "An equipment calibration report" ;
  rdf:value "calibration" .

<https://test.uncefact.org/vocabulary/untp/core/0/attestationTypeCode#certification> a untp-core:attestationTypeCode ;
  rdfs:label "certification" ;
  rdfs:comment "A formal third party certification of conformity" ;
  rdf:value "certification" .

<https://test.uncefact.org/vocabulary/untp/core/0/attestationTypeCode#declaration> a untp-core:attestationTypeCode ;
  rdfs:label "declaration" ;
  rdfs:comment "A self assessed declaration of conformity" ;
  rdf:value "declaration" .

<https://test.uncefact.org/vocabulary/untp/core/0/attestationTypeCode#inspection> a untp-core:attestationTypeCode ;
  rdfs:label "inspection" ;
  rdfs:comment "An Inspection reportÂ " ;
  rdf:value "inspection" .

<https://test.uncefact.org/vocabulary/untp/core/0/attestationTypeCode#testing> a untp-core:attestationTypeCode ;
  rdfs:label "testing" ;
  rdfs:comment "A test report" ;
  rdf:value "testing" .

<https://test.uncefact.org/vocabulary/untp/core/0/attestationTypeCode#validation> a untp-core:attestationTypeCode ;
  rdfs:label "validation" ;
  rdfs:comment "A validation report" ;
  rdf:value "validation" .

<https://test.uncefact.org/vocabulary/untp/core/0/attestationTypeCode#verification> a untp-core:attestationTypeCode ;
  rdfs:label "verification" ;
  rdfs:comment "A verification report" ;
  rdf:value "verification" .

<https://test.uncefact.org/vocabulary/untp/core/0/conformityTopicCode#circularity.content> a untp-core:conformityTopicCode ;
  rdfs:label "Circular content" ;
  rdfs:comment "claims supporting the use of recycled content in products" ;
  rdf:value "circularity.content" .

<https://test.uncefact.org/vocabulary/untp/core/0/conformityTopicCode#circularity.design> a untp-core:conformityTopicCode ;
  rdfs:label "Circular design" ;
  rdfs:comment "claims supporting product design for circularity outcomes" ;
  rdf:value "circularity.design" .

<https://test.uncefact.org/vocabulary/untp/core/0/conformityTopicCode#environment.biodiversity> a untp-core:conformityTopicCode ;
  rdfs:label "Biodiversity" ;
  rdfs:comment "claims supporting improved biodiversity outcomes" ;
  rdf:value "environment.biodiversity" .

<https://test.uncefact.org/vocabulary/untp/core/0/conformityTopicCode#environment.deforestation> a untp-core:conformityTopicCode ;
  rdfs:label "Deforestation" ;
  rdfs:comment "claims supporting native forest restoration" ;
  rdf:value "environment.deforestation" .

<https://test.uncefact.org/vocabulary/untp/core/0/conformityTopicCode#environment.emissions> a untp-core:conformityTopicCode ;
  rdfs:label "GHG emissions" ;
  rdfs:comment "claims supporting GHG emissions reduction" ;
  rdf:value "environment.emissions" .

<https://test.uncefact.org/vocabulary/untp/core/0/conformityTopicCode#environment.energy> a untp-core:conformityTopicCode ;
  rdfs:label "Clean energy" ;
  rdfs:comment "claims supporting clean energy transition" ;
  rdf:value "environment.energy" .

<https://test.uncefact.org/vocabulary/untp/core/0/conformityTopicCode#environment.waste> a untp-core:conformityTopicCode ;
  rdfs:label "Waste reduction" ;
  rdfs:comment "claims supporting waste processing and reduction" ;
  rdf:value "environment.waste" .

<https://test.uncefact.org/vocabulary/untp/core/0/conformityTopicCode#environment.water> a untp-core:conformityTopicCode ;
  rdfs:label "Water usage" ;
  rdfs:comment "claims supporting minimising water usage impact" ;
  rdf:value "environment.water" .

<https://test.uncefact.org/vocabulary/untp/core/0/conformityTopicCode#governance.compliance> a untp-core:conformityTopicCode ;
  rdfs:label "Regulatory compliance" ;
  rdfs:comment "claims supporting regulatory compliance including taxation and community protection" ;
  rdf:value "governance.compliance" .

<https://test.uncefact.org/vocabulary/untp/core/0/conformityTopicCode#governance.ethics> a untp-core:conformityTopicCode ;
  rdfs:label "Ethics" ;
  rdfs:comment "claims supporting ethical conduct and corporate governance" ;
  rdf:value "governance.ethics" .

<https://test.uncefact.org/vocabulary/untp/core/0/conformityTopicCode#governance.transparency> a untp-core:conformityTopicCode ;
  rdfs:label "Transparency" ;
  rdfs:comment "claims supporting transparency and traceability" ;
  rdf:value "governance.transparency" .

<https://test.uncefact.org/vocabulary/untp/core/0/conformityTopicCode#social.community> a untp-core:conformityTopicCode ;
  rdfs:label "Community development" ;
  rdfs:comment "claims supporting local community development" ;
  rdf:value "social.community" .

<https://test.uncefact.org/vocabulary/untp/core/0/conformityTopicCode#social.labour> a untp-core:conformityTopicCode ;
  rdfs:label "Fair work" ;
  rdfs:comment "claims supporting labour rights including fair wages" ;
  rdf:value "social.labour" .

<https://test.uncefact.org/vocabulary/untp/core/0/conformityTopicCode#social.rights> a untp-core:conformityTopicCode ;
  rdfs:label "Human rights" ;
  rdfs:comment "claims supporting human rights and anti-discrimination" ;
  rdf:value "social.rights" .

<https://test.uncefact.org/vocabulary/untp/core/0/conformityTopicCode#social.safety> a untp-core:conformityTopicCode ;
  rdfs:label "Safety" ;
  rdfs:comment "claims supporting process and product safety" ;
  rdf:value "social.safety" .

<https://test.uncefact.org/vocabulary/untp/core/0/encryptionMethodCode#AES> a untp-core:encryptionMethodCode ;
  rdfs:label "AES encrypted" ;
  rdfs:comment "Advanced Encryption Standard (AES)" ;
  rdf:value "AES" .

<https://test.uncefact.org/vocabulary/untp/core/0/encryptionMethodCode#none> a untp-core:encryptionMethodCode ;
  rdfs:label "No encryption" ;
  rdfs:comment "no encryption" ;
  rdf:value "none" .

<https://test.uncefact.org/vocabulary/untp/core/0/hashMethodCode#SHA-1> a untp-core:hashMethodCode ;
  rdfs:label "SHA 160 bit" ;
  rdfs:comment "Secure Hash Algorithm 160 bits" ;
  rdf:value "SHA-1" .

<https://test.uncefact.org/vocabulary/untp/core/0/hashMethodCode#SHA-256> a untp-core:hashMethodCode ;
  rdfs:label "SHA 256 bit" ;
  rdfs:comment "Secure Hash Algorithm 256 bits" ;
  rdf:value "SHA-256" .

<https://test.uncefact.org/vocabulary/untp/core/0/operationalScopeCode#CradleToGate> a untp-core:operationalScopeCode ;
  rdfs:label "Cradle to gate" ;
  rdfs:comment "Includes upstream scope 3 only" ;
  rdf:value "CradleToGate" .

<https://test.uncefact.org/vocabulary/untp/core/0/operationalScopeCode#CradleToGrave> a untp-core:operationalScopeCode ;
  rdfs:label "Cradle to grave" ;
  rdfs:comment "includes full lifecycle (upstream and downstream) scope 3" ;
  rdf:value "CradleToGrave" .

<https://test.uncefact.org/vocabulary/untp/core/0/operationalScopeCode#None> a untp-core:operationalScopeCode ;
  rdfs:label "Excludes scope 3" ;
  rdfs:comment "Scope 1 & 2 only" ;
  rdf:value "None" .

<https://test.uncefact.org/vocabulary/untp/core/0/statusCode#active> a untp-core:statusCode ;
  rdfs:label "Active" ;
  rdfs:comment "The criterion is in active use." ;
  rdf:value "active" .

<https://test.uncefact.org/vocabulary/untp/core/0/statusCode#deprecated> a untp-core:statusCode ;
  rdfs:label "Deprecated" ;
  rdfs:comment "The criterion is deprecated." ;
  rdf:value "deprecated" .

<https://test.uncefact.org/vocabulary/untp/core/0/statusCode#proposed> a untp-core:statusCode ;
  rdfs:label "Proposed" ;
  rdfs:comment "The criterion is proposed" ;
  rdf:value "proposed" .


